---
title: "data605_hw14"
author: "Richard"
date: "5/9/2021"
output: html_document
---
Taylor expansion: f(x)=f(a)+f'(a)(x-a)/1!+f''(a)(x-a)^2/2!+f'''(a)(x-a)^3/3!...

# 1

f(x) = 1/(1-x)  
f'(x) = 1/(1-x)^2
f''(x)= 2/(1-x)^3
f'''(x) = 3/(1-x)^4
when x=0, => 1,1,2,3
taylor: f(x) = 1+1(x)+2(x^2)/2!+2(3)(x^3)/3!...
                
              = 1+x+x^2+x^3...x^n

# 2

f(x) = e^x
f'(x) = e^x
when x=0 => 1,1,1,1,1 (since f(x)==f'(x) or f(x)=e^x)

taylor: f(x) = 1+1(x)+1(x^2)/2!+1(x^3)/3!....

              = 1+x+x^2/2!+x^3/3!...x^n/n!
              
# 3

f(x) =ln(1+x)
f'(x) = 1/(x+1)
f''(x)= -1/(x+1)^2
f'''(x) = 2/(x+1)^3
f''''(x) = -3/(x+1)^4
when x=0 => 0,1,-1,2,-3 (alternates signs)

taylor: f(x)=0+1(x)-1(x^2)/2!+2(x^3)/3!+2(3)(x^4)/4!...
            = x-(x^2)/2+(x^3)/3-(x^4)/4...+(x^n)/n
            