---
title: "hw3"
author: "Richard"
date: "2/15/2021"
output: pdf_document
---


Problem set 1
1) Find Rank of Matrix

A = [[1,2,3,4],                  [[1,2,3,4],                    [[1,2,3,4],               [[1,2,3,4],
    [-1,0,1,3],   -> (r2+r1)/2 -> [0,1,2,7/2],                  [0,1,2,7/2],               [0,1,2,7/2],
    [0,1,-2,1],                   [0,1,-2,1],  -> (r3-r2)/-4 -> [0,0,1,5/8],               [0,0,1,5/8],
    [5,4,-2,-3]]                  [5,4,-2,-3]]                  [5,4,-2,-3]] -> r4-5*r1 -> [0,-6,-17,-23]]
    
    
                [[1,2,3,4],                           [[1,2,3,4],
                [0,1,2,7/2],                          [0,1,2,7/2],
                [0,0,1,5/8],                          [0,0,1,5/8],
-> r4+6*r2 ->   [0,0,-5,-2]]  -> (r4+5*r3)*(8/9) ->   [0,0,0,1]                
    
    
    

Rank of A is 4 

2) Given an mxn matrix where m>n the maximum rank is the number of columns (n) and the minimum rank is 1 given that the matrix is non zero

3) What is the rank of B?

B = [[1,2,1],               [[1,2,1]
     [3,6,3], -> r2-3*r1 ->  [0,0,0],
     [2,4,2]] -> r3-2*r1 ->  [0,0,0]]
    
    rank of B is 1
    
    
Problem set 2
1) Compute EVal and EVector of A

A =[[1,2,3],
    [0,4,5],
    [0,0,6]]
    
det(x*I -A) = 0


=> det([[x-1,-2,-3], = 0 
        [0,x-4,-5],
        [0,0,x-6]])

=> (x-1)((x-4)(x-6)-(-5)(0))-(-2)((0)(x-7)-(-5)(0))+(-3)((0)(0)-(0)(x-4))
   (x-1)((x^2)-10x+24-0)-(-2)(0-0)+(-3)(0-0)
   (x-1)((x^2)-10x+24) = 0
   (x-1)(x-4)(x-6) = 0
   
   x=(1,4,6) are Eigenvalues
   
   
=> for some vector(s) V(x) = [v1,v2,v3]
      ([[x-1,-2,-3],
        [0,x-4,-5], *V(x) = 0
        [0,0,x-6]])   
  
  System of equations:
        (x-1)*V1+(-2)*V2+(-3)*v3 = 0
        0+(x-4)*V2+(-5)*V3 = 0
        0 + 0 +(x-6)V3 = 0
        
=>      (x-1)*V1+(-2)*V2+(-3)*v3 = 0
        (x-4)*V2+(-5)*V3 = 0
        (x-6)V3 = 0
  x = 1
        (0)*V1+(-2)*V2+(-3)*v3 = 0
        (-3)*V2+(-5)*V3 = 0   
        (-5)V3 = 0  => V3 = 0
        => -3*V2+0 = 0 => V2 =0
        => 0*V1 +0 + 0 = 0 => V1 is any number (n)
        
        V(x=1) = [n,0,0]
     
        
  x = 4 
        (3)*V1+(-2)*V2+(-3)*v3 = 0
        (0)*V2+(-5)*V3 = 0
        (-2)V3 = 0 => V3 = 0
        0*V2 +0 = 0 => V2 is any number (n)
        3*V1 -2*V2 + 0 = 0 => 3*V1 = 2V2
        V1 = (2/3)V2 => V1 = (2/3)*n
        
        V(x=4) = [(2/3)*n,n,0]
        
  x = 6 (5)*v1+(-2)*V2+(-3)*v3 = 0
        (2)*v2+(-5)*V3 = 0
        (0)v3 = 0 => v3 is any number (n)
        => 2*v2 = 5*v3 => v2 = (5/2)v3
        => 5*v1 -2(5/2)*v3 -3(v3) = 0
        => 5*v1 -5*v3-3*v3 = 0 => 5*v1 = 8*v3 => v1 = (8/3)v3
        
        V(x=6)=[(8/3)n,(5/2)n,n]
    
        
        
        
        
        
